lam,app

Tibi/Semantics/Eval.lean
@@ -7,18 +7,24 @@ namespace Tibi
 inductive EvalError
 | OutOfBounds_Int64 (n : Int)
 
-inductive Eval (env : Env ctx) : (Expr ctx ty) → Except EvalError Int64 → Prop
-| Const {n : Int} (hLt : n < Int64.size) (hGe : n >= -Int64.size)
-  : Eval env (.Const n) (.ok <| Int64.mk ⟨n, hLt, hGe⟩)
-| ConstErr_lt {n : Int} (h : ¬ n < Int64.size)
-  : Eval env (.Const n) (.error <| .OutOfBounds_Int64 n)
-| ConstErr_ge {n : Int} (h : ¬ n >= -Int64.size)
-  : Eval env (.Const n) (.error <| .OutOfBounds_Int64 n)
-| Var (x : Locals i ctx ty)
-  : Eval env (.Var x) (.ok (env.lookup x))
-
 def EvalError.toString : EvalError → String
 | .OutOfBounds_Int64 n => s!"{n} is out of Int64 bounds, should be satisfied that -2{Nat.toSuperscriptString 63} ≤ n < 2{Nat.toSuperscriptString 63}"
 
 instance : ToString EvalError where
   toString := EvalError.toString
+
+inductive Eval : (Expr ctx ty) → Except EvalError ty.interp → Prop
+| Const {n : Int} (hLt : n < Int64.size) (hGe : n >= -Int64.size)
+  : Eval (.Const n) (.ok <| Int64.mk ⟨n, hLt, hGe⟩)
+| ConstErr_lt {n : Int} (h : ¬ n < Int64.size)
+  : Eval (.Const n) (.error <| .OutOfBounds_Int64 n)
+| ConstErr_ge {n : Int} (h : ¬ n >= -Int64.size)
+  : Eval (.Const n) (.error <| .OutOfBounds_Int64 n)
+-- | Var' (env : Env (α :: .nil)) (a : α.interp) -- {x : Locals 0 (a :: ctx) a}
+--   : Eval (.Var Locals.stop) (.ok <| a)
+| Var (x : Locals k ctx ty) (env : Env ctx)
+  : Eval (.Var x) (.ok <| env.lookup x)
+| Lam (d : Eval e (.ok v))
+  : Eval (.Lam e) (.ok <| fun _ => v)
+| App (d₁ : Eval e₁ (.ok v₁)) (d₂ : Eval e₂ (.ok v₂))
+  : Eval (.App (.Lam e₁) e₂) (.ok <| v₁)
