Tibi/Typing.lean
@@ -7,26 +7,45 @@ namespace Tibi
 
 inductive Typ
 | Int64
+| Fn (a : Typ) (b : Typ)
 deriving DecidableEq
 
 def Typ.toString : Typ → String
-| Int64 => "Int"
+| Int64  => "Int"
+| Fn a b => s!"{a.toString} -> {b.toString}"
 
 instance : ToString Typ where
   toString := Typ.toString
 
 def Ty.toTyp : Ty → Typ
-| int => .Int64
+| int     => .Int64
+| fn a b  => .Fn a.toTyp b.toTyp
+| cls _ b => b.toTyp
 
-inductive HasType (env : Env ctx) : Expr ctx ty → Typ → Prop
-| Int64 {n : Int} (hLt : n < Int64.size) (hGe : n ≥ -Int64.size) : HasType env (.Const n) .Int64
-| Var {x : Locals i ctx ty} : HasType env (.Var x) ty.toTyp
+inductive HasType : Expr ctx ty → Typ → Prop
+| Int64 {n : Int} (hLt : n < Int64.size) (hGe : n ≥ -Int64.size) : HasType (.Const n) .Int64
+| Var {x : Locals i ctx ty} : HasType (.Var x) (Ty.cls ty ty).toTyp
+| Lam (h : HasType e t) : HasType (.Lam e) (.Fn dom t)
+| App (hf : HasType f (.Fn dom ran)) (hv : HasType v dom) : HasType (.App f v) ran
 
-def Expr.typeCheck (env : Env ctx) : (e : Expr ctx ty) → {{ t | HasType env e t }}
+def Expr.typeCheck : (e : Expr ctx ty) → {{ t | HasType e t }}
 | .Const n =>
     if h : -Int64.size ≤ n ∧ n < Int64.size then
       .found .Int64 <| .Int64 h.right h.left
     else
       .unknown
 | .Var _ =>
-      .found ty.toTyp .Var
+    .found _ .Var
+| .Lam e =>
+    match e.typeCheck with
+    | .found t h => .found (.Fn .Int64 t) <| .Lam h
+    | .unknown   => .unknown
+| .App f v =>
+    match f.typeCheck, v.typeCheck with
+    | .found (.Fn a b) hf, .found a' hv =>
+        if h : a = a' then
+          .found b <| .App hf (h ▸ hv)
+        else
+          .unknown
+    | _, _ => .unknown
+-- | _ => .unknown
