Tibi/Interpreter.lean
@@ -5,12 +5,26 @@ import Tibi.Util
 
 namespace Tibi
 
-def Expr.eval (env : Env ctx) : (e : Expr ctx ty) → {{ r | Eval env e r }}
-| .Const n =>
+def Expr.eval (env : Env ctx) : {ty : Ty} → (e : Expr ctx ty) → ty.dom → {{ r | Eval e r }}
+| _, .Const n, _ =>
     if h : (-Int64.size : Int) ≤ n ∧ n < Int64.size then
-      .found (.ok <| Int64.mk ⟨n, h.right, h.left⟩) <| Eval.Const h.right h.left
+      .found (.ok <| Int64.mk ⟨n, h.right, h.left⟩) <| .Const h.right h.left
     else
       Decidable.not_and_iff_or_not_not.mp h |>.by_cases
         (fun h => .found (.error <| .OutOfBounds_Int64 n) <| Eval.ConstErr_ge h)
         (fun h => .found (.error <| .OutOfBounds_Int64 n) <| Eval.ConstErr_lt h)
-| .Var x => .found (.ok <| env.lookup x) <| Eval.Var x
+| _, .Var x, _ =>
+    .found (.ok <| env.lookup x) <| .Var x env
+| _, .Lam e', x =>
+    match e'.eval (x :: env) x with
+    | .found (.ok v) h => .found (.ok <| fun _ => v) <| .Lam h
+    | .unknown => .unknown
+| .int, .App (dom := .int) (.Lam e₁) e₂, _ =>
+    match e₂.eval env () with
+    | .found (.ok v) h₂ =>
+        match e₁.eval (v :: env) v with
+        | .found (.ok v) h₁ =>
+            .found (.ok <| v) <| .App h₁ h₂
+        | _ => .unknown
+    | _ => .unknown
+| _, _, _ => .unknown
