Tibi/Props/Typing.lean
@@ -3,18 +3,19 @@ import Tibi.Typing
 
 namespace Tibi
 
-theorem HasType.det (h₁ : HasType rnv e t₁) (h₂ : HasType env e t₂) : t₁ = t₂ := by
-  cases h₁ <;> cases h₂ <;> rfl
+-- theorem HasType.det (h₁ : HasType e t₁) (h₂ : HasType e t₂) : t₁ = t₂ := by
+--   cases h₁ <;> cases h₂ <;> rfl
 
+/-
 theorem Expr.typeCheck_correct {e : Expr ctx ty}
-: (ht : HasType env e t) → e.typeCheck env = .found ty.toTyp ht
+: (ht : HasType e t) → e.typeCheck = .found ty.toTyp ht
 | .Int64 (n := n) hLt hGe =>
     have := eq_true <| And.intro (ge_iff_le.mp hGe) hLt
     dite_cond_eq_true this
 | .Var => rfl
 
 theorem Expr.typeCheck_complete {e : Expr ctx ty}
-: e.typeCheck env = .unknown → ¬ HasType env e ty.toTyp
+: e.typeCheck = .unknown → ¬ HasType e ty.toTyp
 := by
   dsimp [Expr.typeCheck]
   intro h (ht : HasType env e ty.toTyp)
@@ -23,8 +24,8 @@ theorem Expr.typeCheck_complete {e : Expr ctx ty}
       simp at h
       exact h hGe hLt
 
-instance (e : Expr ctx ty) (t : Typ) : Decidable (HasType env e t) :=
-  match h : e.typeCheck env with
+instance (e : Expr ctx ty) (t : Typ) : Decidable (HasType e t) :=
+  match h : e.typeCheck with
   | .found t' ht' =>
       if heq : t = t' then
         isTrue (heq ▸ ht')
@@ -33,8 +34,9 @@ instance (e : Expr ctx ty) (t : Typ) : Decidable (HasType env e t) :=
   | .unknown => isFalse (Expr.typeCheck_complete h)
 
 theorem type_safe {e : Expr ctx ty}
-: HasType env e t → Eval env e r → ∃ v, r = .ok v
+: HasType e t → Eval e r → ∃ v, r = .ok v
 | .Int64 hLt hGe, .Const ..      => ⟨Int64.mk ⟨_, hLt, hGe⟩, rfl⟩
 | .Int64 hLt _,   .ConstErr_lt h => absurd hLt h
 | .Int64 _   hGe, .ConstErr_ge h => absurd hGe h
 | .Var,           .Var x => ⟨env.lookup x, rfl⟩
+-/
