Tibi/Syntax/Expr.lean
@@ -5,13 +5,25 @@ namespace Tibi
 
 inductive Ty where
 | int
+| fn (a b : Ty)
+| cls (a b : Ty)
 
 @[reducible]
 def Ty.interp : Ty → Type
-| int => Int64
+| int    => Int64
+| fn a b => a.interp → b.interp
+| cls _ b => b.interp
+
+@[reducible]
+def Ty.dom : Ty → Type
+| int => Unit
+| fn a _ => a.interp
+| cls a _ => a.interp
 
 def Ty.toString : Ty → String
-| int => "Int"
+| int    => "Int"
+| fn a b => s!"{a.toString} -> {b.toString}"
+| cls _ b => s!"{b.toString}"
 
 instance : ToString Ty where
   toString := Ty.toString
@@ -29,11 +41,15 @@ instance : ToString (Locals n ctx ty) where
 
 inductive Expr : Vec Ty n → Ty → Type where
 | Const : Int → Expr ctx .int
-| Var   : Locals i ctx ty → Expr ctx ty
+| Var   : Locals i ctx ty → Expr ctx (.cls ty ty)
+| Lam   : Expr (dom :: ctx) (.cls dom ran) → Expr ctx (.fn dom ran)
+| App   : Expr ctx (.fn dom ran) → Expr ctx dom → Expr ctx ran
 
 def Expr.toString : Expr ctx ty → String
 | Const n => s!"<Const {n}>"
 | Var x   => s!"<Var {x} @{ty}>"
+| Lam e   => s!"<Lam {e.toString}>"
+| App e₁ e₂ => s!"<App {e₁.toString} {e₂.toString}>"
 
 instance : ToString (Expr ctx ty) where
   toString := Expr.toString
